specs/Spec.CRC32.Bits.fst
@@ -2,24 +2,24 @@ module Spec.CRC32.Bits
 
 module BV = FStar.BitVector
 module Math = FStar.Math.Lemmas
-module Seq = FStar.Seq
 module U32 = FStar.UInt32
 module UInt = FStar.UInt
 
+open FStar.Seq
 open Lib.Seq
 open Lib.UInt
 
 #set-options "--z3rlimit 200 --z3seed 1 --fuel 1 --ifuel 1"
-let poly_xor_zero_prefix (#n: nat{n >= 32}) (a: BV.bv_t n) (m: nat{m > 0}): Lemma
-  (ensures forall (i: nat{i > 0}).
+let poly_xor_zero_prefix (#n: nat{n >= 32}) (a: BV.bv_t n) (m: pos): Lemma
+  (ensures forall (i: pos).
     i < Seq.length (zero_vec_l m a) ==>
-    Seq.index (poly_xor (zero_vec_l m a)) i ==
-    Seq.index (poly_xor (zero_vec_l (m - 1) a)) (i - 1)) = ()
+    (poly_xor (zero_vec_l m a)).[i] ==
+    (poly_xor (zero_vec_l (m - 1) a)).[i - 1]) = ()
 
-let zero_vec_l_aux (#n: nat{n > 0}) (a: BV.bv_t n) (m: nat{m > 0}): Lemma
-  (ensures forall (i: nat{i > 0}).
+let zero_vec_l_aux (#n: pos) (a: BV.bv_t n) (m: pos): Lemma
+  (ensures forall (i: pos).
     i < Seq.length (zero_vec_l m a) ==>
-   Seq.index (zero_vec_l m a) i == Seq.index (zero_vec_l (m - 1) a) (i - 1)) = ()
+    (zero_vec_l m a).[i] == (zero_vec_l (m - 1) a).[i - 1]) = ()
 
 let rec poly_xor_zero_vec_l (#n: nat{n >= 32}) (a: BV.bv_t n) (m: nat): Lemma
   (ensures zero_vec_l m (poly_xor a) == poly_xor (zero_vec_l m a)) =
@@ -36,42 +36,22 @@ let rec poly_xor_zero_vec_l (#n: nat{n >= 32}) (a: BV.bv_t n) (m: nat): Lemma
     zero_vec_l_aux (poly_xor a) m;
     poly_xor_zero_vec_l a (m - 1);
     calc (==) {
-      Seq.index c 0;
+      c.[0];
       =={}
-      Seq.index ((zero_vec_l m a) -@ p') 0;
+      ((zero_vec_l m a) -@ p').[0];
       =={
-        assert(Seq.index (zero_vec_l m a) 0 == false);
-        assert(Seq.index p 0 == false);
-        assert(Seq.index p' 0 == false)
+        assert((zero_vec_l m a).[0] == false);
+        assert(p.[0] == false);
+        assert(p'.[0] == false)
       }
       false;
     };
-    assert(Seq.index b 0 == Seq.index c 0);
+    assert(b.[0] == c.[0]);
     assert(Seq.equal b c)
 
 let poly_xor_sub_eq (#n: nat{n > 32}) (a: BV.bv_t n): Lemma
   (ensures poly_xor #(n - 1) (unsnoc a) == unsnoc (a -@ (poly n))) =
   assert(Seq.equal (poly_xor #(n - 1) (unsnoc a)) (unsnoc (a -@ (poly n))))
-
-let logxor_zero_eq (#n: nat{n > 0}) (a: BV.bv_t n): Lemma
-  (ensures (BV.logxor_vec a (BV.zero_vec #n)) == a)
-  [SMTPat (BV.logxor_vec a (BV.zero_vec #n))] =
-    let z = BV.zero_vec #n in
-    let x = BV.logxor_vec a z in
-    assert_norm(forall (i: nat) (v: BV.bv_t n). i < n ==> Seq.index v i = Seq.index v i <> false);
-    assert_norm(Seq.equal x a)
-
-let logxor_eq_zero (#n: nat{n > 0}) (a b: BV.bv_t n): Lemma
-  (requires a == b)
-  (ensures BV.logxor_vec a b == BV.zero_vec #n)
-  [SMTPat (BV.logxor_vec #n a b)] =
-  assert(Seq.equal (BV.logxor_vec a b) (BV.zero_vec #n))
-
-let logxor_vec_assoc (#n: nat{n > 0}) (a b c: BV.bv_t n): Lemma
-  (ensures BV.logxor_vec (BV.logxor_vec a b) c == BV.logxor_vec a (BV.logxor_vec b c))
-  [SMTPat (BV.logxor_vec (BV.logxor_vec a b) c); 
-   SMTPat (BV.logxor_vec a (BV.logxor_vec b c))] =
-  assert(Seq.equal (BV.logxor_vec (BV.logxor_vec a b) c) (BV.logxor_vec a (BV.logxor_vec b c)))
 
 let poly_xor_aux (#n: nat{n >= 32}) (a b: BV.bv_t n): Lemma
   (ensures (poly_xor a) +@ (poly_xor b) == a +@ b) =
@@ -180,7 +160,7 @@ let rec poly_mod_add #n a b =
 let rec poly_mod_zero_prefix #n a m =
   assert(Seq.equal (zero_vec_l #(n - 1) m (unsnoc a)) (unsnoc (zero_vec_l m a)));
   if n = 33 then
-    if Seq.index a (n - 1) then
+    if a.[n - 1] then
       calc (==) {
         poly_mod (zero_vec_l m (poly_mod a));
         =={assert(Seq.equal (poly_mod a) (poly_xor #(n - 1) (unsnoc a)))}
@@ -205,7 +185,7 @@ let rec poly_mod_zero_prefix #n a m =
         poly_mod (zero_vec_l m a);
       }
   else
-    if Seq.index a (n - 1) then
+    if a.[n - 1] then
       calc (==) {
         poly_mod (zero_vec_l m (poly_mod a));
         =={}
@@ -266,7 +246,7 @@ let rec poly_mod_zero_suffix #n a m =
         poly_mod a;
       }
 
-private let rec logand_mask_aux (a: nat{a > 0}) (n: nat{n >= a}): Lemma
+private let rec logand_mask_aux (a: pos) (n: nat{n >= a}): Lemma
   (requires (pow2 a) - 1 < pow2 n)
   (ensures forall i. 
     (i >= n - a ==> UInt.nth #n ((pow2 a) - 1) i == true) /\
@@ -287,28 +267,28 @@ let large_table_val_aux i nzeros p p' p'' =
    let vpand = UInt.to_vec (U32.v (U32.logand p 0xFFul)) in
    logand_mask_aux 8 32;
    assert(forall i.
-     i < 32 - 8 ==> Seq.index vpand i == false /\
-     i >= 32 - 8 ==> Seq.index vpand i == Seq.index vp i);
+     i < 32 - 8 ==> vpand.[i] == false /\
+     i >= 32 - 8 ==> vpand.[i] == vp.[i]);
    assert(vp' == poly_mod (zero_vec_l 8 vpand));
 
    assert(forall i.
-     i >= 8 ==> Seq.index vp'' i == Seq.index vp (i - 8) /\
-     i < 8 ==> Seq.index vp'' i == false);
+     i >= 8 ==> vp''.[i] == vp.[i - 8] /\
+     i < 8 ==> vp''.[i] == false);
    poly_mod_zero_suffix vp'' 8;
    assert(vp'' == poly_mod (zero_vec_r 8 vp''));
 
    assert(forall i. {:pattern Seq.index (zero_vec_l 8 vpand) i}
-     (i >= 40 - 8 ==> Seq.index (zero_vec_l 8 vpand) i == Seq.index vp (i - 8)) /\
-     (i < 40 - 8 ==> Seq.index (zero_vec_l 8 vpand) i == false));
+     (i >= 40 - 8 ==> (zero_vec_l 8 vpand).[i] == vp.[i - 8]) /\
+     (i < 40 - 8 ==> (zero_vec_l 8 vpand).[i] == false));
 
    assert(forall i. {:pattern Seq.index (zero_vec_r 8 vp'') i}
-     (i < 8 \/ i >= 32 ==> Seq.index (zero_vec_r 8 vp'') i == false) /\
-     (i >= 8 /\ i < 32 ==> Seq.index (zero_vec_r 8 vp'') i == Seq.index vp (i - 8)));
+     (i < 8 \/ i >= 32 ==> (zero_vec_r 8 vp'').[i] == false) /\
+     (i >= 8 /\ i < 32 ==> (zero_vec_r 8 vp'').[i] == vp.[i - 8]));
 
    let sum = (zero_vec_l 8 vpand) +@ (zero_vec_r 8 vp'') in
    assert(forall i. {:pattern Seq.index sum i}
-     (i < 8 ==> Seq.index sum i == false) /\
-     (i >= 8 ==> Seq.index sum i == Seq.index vp (i - 8)));
+     (i < 8 ==> sum.[i] == false) /\
+     (i >= 8 ==> sum.[i] == vp.[i - 8]));
    assert(Seq.equal sum (zero_vec_l 8 vp));
    
    poly_mod_add (zero_vec_l 8 vpand) (zero_vec_r 8 vp'');
@@ -320,7 +300,58 @@ let large_table_val_aux i nzeros p p' p'' =
    zero_vec_l_app vi nzeros 8;
    assert(vp' +@ vp'' == poly_mod (zero_vec_l (nzeros + 8) vi))
 
-open FStar.Seq
+let rec data_bits_rev_app_one (s: Seq.seq U8.t) (t: U8.t): Lemma
+  (ensures UInt.to_vec (U8.v t) @| data_bits_rev s == data_bits_rev (s @| create 1 t))
+  (decreases length s) =
+  match length s with
+  | 0 -> ()
+  | _ ->
+    calc (==) {
+      UInt.to_vec (U8.v t) @| data_bits_rev s;
+      =={}
+      UInt.to_vec (U8.v t) @| (data_bits_rev (tail s)) @| UInt.to_vec (U8.v (head s));
+      =={
+        append_assoc
+          (UInt.to_vec (U8.v t))
+          (data_bits_rev (tail s))
+          (UInt.to_vec (U8.v (head s)))
+      }
+      (UInt.to_vec (U8.v t) @| (data_bits_rev (tail s))) @| UInt.to_vec (U8.v (head s)); 
+      =={data_bits_rev_app_one (tail s) t}
+      data_bits_rev ((tail s) @| create 1 t) @| UInt.to_vec (U8.v (head s));
+      =={
+        assert(Seq.equal ((tail s) @| create 1 t) (tail (s @| create 1 t)))
+      }
+      data_bits_rev (tail (s @| create 1 t)) @| UInt.to_vec (U8.v (head s));
+      =={}
+      data_bits_rev (s @| create 1 t);
+    }
+
+let rec data_bits_rev_app s1 s2 =
+  match length s2 with
+  | 0 -> assert(Seq.equal ((data_bits_rev s2) @| data_bits_rev s1) (data_bits_rev s1))
+  | 1 ->
+    data_bits_rev_app_one s1 (head s2);
+    assert(Seq.equal (s1 @| create 1 (head s2)) (s1 @| s2))
+  | _ ->
+    calc (==) {
+      (data_bits_rev s2) @| data_bits_rev s1;
+      =={
+        append_assoc
+          (data_bits_rev (tail s2))
+          (UInt.to_vec (U8.v (head s2)))
+          (data_bits_rev s1)
+      }
+      (data_bits_rev (tail s2)) @| ((UInt.to_vec (U8.v (head s2))) @| data_bits_rev s1);
+      =={data_bits_rev_app_one s1 (head s2)}
+      (data_bits_rev (tail s2)) @| data_bits_rev (s1 @| create 1 (head s2));
+      =={data_bits_rev_app (s1 @| create 1 (head s2)) (tail s2)}
+      data_bits_rev ((s1 @| (create 1 (head s2))) @| (tail s2));
+      =={append_assoc s1 (create 1 (head s2)) (tail s2)}
+      data_bits_rev (s1 @| ((create 1 (head s2)) @| (tail s2)));
+      =={assert(Seq.equal s2 (create 1 (head s2) @| tail s2))}
+      data_bits_rev (s1 @| s2);
+    }
 
 val crc32_data_to_bits_append':
     #n: crc32_buf_len
@@ -402,6 +433,176 @@ let rec crc32_data_to_bits_append' #n m1 m2 s1 s2 buf =
 let crc32_data_to_bits_append m1 m2 s1 s2 =
   crc32_data_to_bits_append' #0 m1 m2 s1 s2 (Seq.empty #bool)
 
+let rec crc32_data_to_bits_rev n data =
+  match n with
+  | 1 ->
+    calc (==) {
+      crc32_data_to_bits n data;
+      =={}
+      zero_vec_l 8 (BV.ones_vec #32 +@ (BV.zero_vec #24 @| UInt.to_vec (U8.v data.[0])));
+      =={
+        assert(Seq.equal
+          (UInt.to_vec (U8.v data.[0]))
+          (data_bits_rev data))
+      }
+      zero_vec_l 8 (BV.ones_vec #32 +@ (BV.zero_vec #24 @| data_bits_rev data));
+      =={
+        assert(Seq.equal
+          (zero_vec_l 8 (BV.ones_vec #32 +@
+            (BV.zero_vec #24 @| data_bits_rev data)))
+          ((zero_vec_l 8 (BV.ones_vec #32)) +@
+            (zero_vec_l 8 (BV.zero_vec #24 @| data_bits_rev data))))
+      }
+      (zero_vec_l 8 (BV.ones_vec #32)) +@
+      (zero_vec_l 8 (BV.zero_vec #24 @| data_bits_rev data));
+      =={
+        assert(Seq.equal
+          (BV.zero_vec #24 @| data_bits_rev data)
+          (zero_vec_l 24 (data_bits_rev data)))
+      }
+      (zero_vec_l 8 (BV.ones_vec #32)) +@
+      (zero_vec_l 8 (zero_vec_l 24 (data_bits_rev data)));
+      =={zero_vec_l_app (data_bits_rev data) 24 8}
+      (zero_vec_l 8 (BV.ones_vec #32)) +@
+      (zero_vec_l 32 (data_bits_rev data));
+    }
+  | _ ->
+    let data' = Seq.slice data 0 (n - 1) in
+    let t = Seq.create 1 (Seq.last data) in
+    calc (==) {
+      zero_vec_l 40 (data_bits_rev data') +@
+      zero_vec_l #(n * 8) 32
+        (UInt.to_vec (U8.v (Seq.last data)) @| BV.zero_vec #((n - 1) * 8));
+      =={
+        assert(Seq.equal
+          (zero_vec_l 40 (data_bits_rev data'))
+          (zero_vec_l #(n * 8) 32 (BV.zero_vec #8 @|data_bits_rev data')))
+      }
+      zero_vec_l 32 (BV.zero_vec #8 @| data_bits_rev data') +@
+      zero_vec_l #(n * 8) 32 (
+        UInt.to_vec (U8.v (Seq.last data)) @| BV.zero_vec #((n - 1) * 8));
+      =={
+        assert(Seq.equal
+          (zero_vec_l 32 (BV.zero_vec #8 @| data_bits_rev data') +@
+           zero_vec_l #(n * 8) 32 (
+             UInt.to_vec (U8.v (Seq.last data)) @| BV.zero_vec #((n - 1) * 8)))
+          (zero_vec_l #(n * 8) 32 (
+            (BV.zero_vec #8 @| data_bits_rev data') +@
+            (UInt.to_vec (U8.v (Seq.last data)) @| BV.zero_vec #((n - 1) * 8)))))
+      }
+      zero_vec_l #(n * 8) 32 (
+        (BV.zero_vec #8 @| data_bits_rev data') +@
+        (UInt.to_vec (U8.v (Seq.last data)) @| BV.zero_vec #((n - 1) * 8)));
+      =={
+        assert(Seq.equal
+          (zero_vec_l #(n * 8) 32 (
+            (BV.zero_vec #8 @| data_bits_rev data') +@
+            (UInt.to_vec (U8.v (Seq.last data)) @| BV.zero_vec #((n - 1) * 8))))
+          (zero_vec_l #(n * 8) 32
+            (UInt.to_vec (U8.v (Seq.last data)) @| data_bits_rev data')))
+      }
+      zero_vec_l #(n * 8) 32
+        (UInt.to_vec (U8.v (Seq.last data)) @| data_bits_rev data');
+      =={
+        data_bits_rev_app_one data' (Seq.last data);
+        assert(Seq.equal (data' @| (create 1 (last data))) data)
+      }
+      zero_vec_l 32 (data_bits_rev data);
+    };
+    calc (==) {
+      crc32_data_to_bits n data;
+      =={
+        crc32_data_to_bits_append (n - 1) 1 data' t;
+        assert(Seq.equal (data' @| t) data)
+      }
+      crc32_data_to_bits_cont 1 t (crc32_data_to_bits (n - 1) data');
+      =={}
+      crc32_append_8bit (crc32_data_to_bits (n - 1) data') (Seq.last data);
+      =={}
+      zero_vec_l 8
+        ((crc32_data_to_bits (n - 1) data') +@ 
+        ((BV.zero_vec #24) @|
+         (UInt.to_vec (U8.v (Seq.last data))) @|
+         (BV.zero_vec #((n - 1) * 8))));
+      =={
+        assert(Seq.equal
+          ((BV.zero_vec #24) @|
+           (UInt.to_vec (U8.v (Seq.last data))) @|
+           (BV.zero_vec #((n - 1) * 8)))
+          (zero_vec_l #(n * 8) 24
+           (UInt.to_vec (U8.v (Seq.last data)) @| (BV.zero_vec #((n - 1) * 8)))))
+      }
+      zero_vec_l 8
+        ((crc32_data_to_bits (n - 1) data') +@ 
+        (zero_vec_l #(n * 8) 24
+         (UInt.to_vec (U8.v (Seq.last data)) @| BV.zero_vec #((n - 1) * 8))));
+      =={
+        assert(Seq.equal
+          (zero_vec_l 8
+            ((crc32_data_to_bits (n - 1) data') +@ 
+            (zero_vec_l #(n * 8) 24
+              (UInt.to_vec (U8.v (Seq.last data)) @|
+              (BV.zero_vec #((n - 1) * 8))))))
+          ((zero_vec_l 8 (crc32_data_to_bits (n - 1) data')) +@
+           (zero_vec_l 8 (zero_vec_l #(n * 8) 24
+             (UInt.to_vec (U8.v (Seq.last data)) @| BV.zero_vec #((n - 1) * 8))))))
+      }
+      (zero_vec_l 8 (crc32_data_to_bits (n - 1) data')) +@
+      (zero_vec_l 8 (zero_vec_l #(n * 8) 24
+        (UInt.to_vec (U8.v (Seq.last data)) @| BV.zero_vec #((n - 1) * 8))));
+      =={
+        zero_vec_l_app #(n * 8)
+          (UInt.to_vec (U8.v (Seq.last data)) @| BV.zero_vec #((n - 1) * 8))
+          24 8
+      }
+      (zero_vec_l 8 (crc32_data_to_bits (n - 1) data')) +@
+      zero_vec_l #(n * 8) 32
+        (UInt.to_vec (U8.v (Seq.last data)) @| BV.zero_vec #((n - 1) * 8));
+      =={crc32_data_to_bits_rev (n - 1) data'}
+      (zero_vec_l 8
+        ((zero_vec_l ((n - 1) * 8) (BV.ones_vec #32)) +@
+          (zero_vec_l 32 (data_bits_rev data')))) +@
+      zero_vec_l #(n * 8) 32
+        (UInt.to_vec (U8.v (Seq.last data)) @| BV.zero_vec #((n - 1) * 8));
+      =={
+        assert(Seq.equal
+          (zero_vec_l 8
+            ((zero_vec_l ((n - 1) * 8) (BV.ones_vec #32)) +@
+            (zero_vec_l 32 (data_bits_rev data'))))
+          ((zero_vec_l 8 (zero_vec_l ((n - 1) * 8) (BV.ones_vec #32))) +@
+           (zero_vec_l 8 (zero_vec_l 32 (data_bits_rev data')))))
+      }
+      ((zero_vec_l 8 (zero_vec_l ((n - 1) * 8) (BV.ones_vec #32))) +@
+        (zero_vec_l 8 (zero_vec_l 32 (data_bits_rev data')))) +@
+      zero_vec_l #(n * 8) 32
+        (UInt.to_vec (U8.v (Seq.last data)) @| BV.zero_vec #((n - 1) * 8));
+      =={
+        zero_vec_l_app (BV.ones_vec #32) ((n - 1) * 8) 8;
+        zero_vec_l_app (data_bits_rev data') 32 8
+      }
+      (zero_vec_l (n * 8) (BV.ones_vec #32) +@
+       zero_vec_l 40 (data_bits_rev data')) +@
+      zero_vec_l #(n * 8) 32
+        (UInt.to_vec (U8.v (Seq.last data)) @| BV.zero_vec #((n - 1) * 8));
+      =={
+        assert(Seq.equal
+          ((zero_vec_l (n * 8) (BV.ones_vec #32) +@
+            zero_vec_l 40 (data_bits_rev data')) +@
+          zero_vec_l #(n * 8) 32
+            (UInt.to_vec (U8.v (Seq.last data)) @| BV.zero_vec #((n - 1) * 8)))
+          (zero_vec_l (n * 8) (BV.ones_vec #32) +@
+            (zero_vec_l 40 (data_bits_rev data') +@
+            zero_vec_l #(n * 8) 32
+            (UInt.to_vec (U8.v (Seq.last data)) @| BV.zero_vec #((n - 1) * 8)))))
+      }
+      zero_vec_l (n * 8) (BV.ones_vec #32) +@
+      (zero_vec_l 40 (data_bits_rev data') +@
+      zero_vec_l #(n * 8) 32
+        (UInt.to_vec (U8.v (Seq.last data)) @| BV.zero_vec #((n - 1) * 8)));
+      =={}
+      (zero_vec_l (n * 8) (BV.ones_vec #32)) +@ zero_vec_l 32 (data_bits_rev data);
+    }
+
 #set-options "--z3rlimit 200 --fuel 0 --ifuel 0"
 let crc32_data_to_bits_32bit_aux (a b c d: U8.t) (buf: BV.bv_t 64): Lemma
   (requires buf ==
@@ -409,10 +610,10 @@ let crc32_data_to_bits_32bit_aux (a b c d: U8.t) (buf: BV.bv_t 64): Lemma
       #0 (Seq.empty #bool) a) b) c) d))
   (ensures forall (i: nat{i < 64}). {:pattern Seq.index buf i}
     (i >= 56 ==> Seq.index buf i == (UInt.nth (U8.v a) (i - 56) <> true)) /\
-    (i >= 48 /\ i < 56 ==> Seq.index buf i == (UInt.nth (U8.v b) (i - 48) <> true)) /\
-    (i >= 40 /\ i < 48 ==> Seq.index buf i == (UInt.nth (U8.v c) (i - 40) <> true)) /\
-    (i >= 32 /\ i < 40 ==> Seq.index buf i == (UInt.nth (U8.v d) (i - 32) <> true)) /\
-    (i < 32 ==> Seq.index buf i == false)) =
+    (i >= 48 /\ i < 56 ==> buf.[i] == (UInt.nth (U8.v b) (i - 48) <> true)) /\
+    (i >= 40 /\ i < 48 ==> buf.[i] == (UInt.nth (U8.v c) (i - 40) <> true)) /\
+    (i >= 32 /\ i < 40 ==> buf.[i] == (UInt.nth (U8.v d) (i - 32) <> true)) /\
+    (i < 32 ==> buf.[i] == false)) =
   let s = crc32_dword_seq a b c d in
   let a' = UInt.to_vec (U8.v a) in
   let b' = UInt.to_vec (U8.v b) in
@@ -428,29 +629,29 @@ let crc32_data_to_bits_32bit_aux (a b c d: U8.t) (buf: BV.bv_t 64): Lemma
   let dbuf = zero_vec_l 8 (cbuf +@ dpad) in
   
   assert(forall (i: nat{i < 40}). {:pattern Seq.index abuf i}
-    (i >= 32 ==> Seq.index abuf i == (Seq.index a' (i - 32) <> true)) /\
-    (i >= 8 /\ i < 32 ==> Seq.index abuf i == true) /\
-    (i < 8 ==> Seq.index abuf i == false));
+    (i >= 32 ==> abuf.[i] == (Seq.index a' (i - 32) <> true)) /\
+    (i >= 8 /\ i < 32 ==> abuf.[i] == true) /\
+    (i < 8 ==> abuf.[i] == false));
 
   assert(forall (i: nat{i < 48}). {:pattern Seq.index bbuf i}
-    (i >= 40 ==> Seq.index bbuf i == (Seq.index a' (i - 40) <> true)) /\
-    (i >= 32 /\ i < 40 ==> Seq.index bbuf i == (Seq.index b' (i - 32) <> true)) /\
-    (i >= 16 /\ i < 32 ==> Seq.index bbuf i == true) /\
-    (i < 16 ==> Seq.index bbuf i == false));
+    (i >= 40 ==> bbuf.[i] == (a'.[i - 40] <> true)) /\
+    (i >= 32 /\ i < 40 ==> bbuf.[i] == (b'.[i - 32] <> true)) /\
+    (i >= 16 /\ i < 32 ==> bbuf.[i] == true) /\
+    (i < 16 ==> bbuf.[i] == false));
 
   assert(forall (i: nat{i < 56}). {:pattern Seq.index cbuf i}
-    (i >= 48 ==> Seq.index cbuf i == (Seq.index a' (i - 48) <> true)) /\
-    (i >= 40 /\ i < 48 ==> Seq.index cbuf i == (Seq.index b' (i - 40) <> true)) /\
-    (i >= 32 /\ i < 40 ==> Seq.index cbuf i == (Seq.index c' (i - 32) <> true)) /\
-    (i >= 24 /\ i < 32 ==> Seq.index cbuf i == true) /\
-    (i < 24 ==> Seq.index cbuf i == false));
+    (i >= 48 ==> Seq.index cbuf i == (a'.[i - 48] <> true)) /\
+    (i >= 40 /\ i < 48 ==> cbuf.[i] == (b'.[i - 40] <> true)) /\
+    (i >= 32 /\ i < 40 ==> cbuf.[i] == (c'.[i - 32] <> true)) /\
+    (i >= 24 /\ i < 32 ==> cbuf.[i] == true) /\
+    (i < 24 ==> cbuf.[i] == false));
 
   assert(forall (i: nat{i < 64}). {:pattern Seq.index dbuf i}
-    (i >= 56 ==> Seq.index dbuf i == (Seq.index a' (i - 56) <> true)) /\
-    (i >= 48 /\ i < 56 ==> Seq.index dbuf i == (Seq.index b' (i - 48) <> true)) /\
-    (i >= 40 /\ i < 48 ==> Seq.index dbuf i == (Seq.index c' (i - 40) <> true)) /\
-    (i >= 32 /\ i < 40 ==> Seq.index dbuf i == (Seq.index d' (i - 32) <> true)) /\
-    (i < 32 ==> Seq.index dbuf i == false))
+    (i >= 56 ==> dbuf.[i] == (a'.[i - 56] <> true)) /\
+    (i >= 48 /\ i < 56 ==> dbuf.[i] == (b'.[i - 48] <> true)) /\
+    (i >= 40 /\ i < 48 ==> dbuf.[i] == (c'.[i - 40] <> true)) /\
+    (i >= 32 /\ i < 40 ==> dbuf.[i] == (d'.[i - 32] <> true)) /\
+    (i < 32 ==> dbuf.[i] == false))
 
 private unfold let xor_status
   (#n: nat{n > 32})
@@ -460,8 +661,7 @@ private unfold let xor_status
   (a: U8.t) 
   (i: nat{i >= offset /\ i < offset + n})
   (j: nat{i - j >= 0 /\ i - j < 8}) =
-    Seq.index res i ==
-    (Seq.index (UInt.to_vec (U8.v a)) (i - j) <> Seq.index buf (i - offset))
+    res.[i] == ((UInt.to_vec (U8.v a)).[i - j] <> buf.[i - offset])
 
 let crc32_data_to_bits_32bit_aux'
   (#n: nat{n > 32})
@@ -472,12 +672,12 @@ let crc32_data_to_bits_32bit_aux'
       buf a) b) c) d
   }): Lemma
   (ensures forall (i: nat{i < 32 + n}).
-    (i >= 64 ==> Seq.index buf' i == Seq.index buf (i - 32)) /\
+    (i >= 64 ==> buf'.[i] == buf.[i - 32]) /\
     (i >= 56 /\ i < 64 ==> xor_status buf' buf a i 56) /\
     (i >= 48 /\ i < 56 ==> xor_status buf' buf b i 48) /\
     (i >= 40 /\ i < 48 ==> xor_status buf' buf c i 40) /\
     (i >= 32 /\ i < 40 ==> xor_status buf' buf d i 32) /\
-    (i < 32 ==> Seq.index buf' i == false)) =
+    (i < 32 ==> buf'.[i] == false)) =
   let a' = UInt.to_vec (U8.v a) in
   let b' = UInt.to_vec (U8.v b) in
   let c' = UInt.to_vec (U8.v c) in
@@ -493,33 +693,33 @@ let crc32_data_to_bits_32bit_aux'
   let dbuf = zero_vec_l 8 (cbuf +@ dpad) in
 
   assert(forall (i: nat{i < n + 8}). {:pattern Seq.index abuf i}
-    (i >= 40 ==> Seq.index abuf i == Seq.index buf (i - 8)) /\
+    (i >= 40 ==> abuf.[i] == buf.[i - 8]) /\
     (i >= 32 /\ i < 40 ==> xor_status #n #8 abuf buf a i 32) /\
-    (i >= 8 /\ i < 32 ==> Seq.index abuf i == Seq.index buf (i - 8)) /\
-    (i < 8 ==> Seq.index abuf i == false));
+    (i >= 8 /\ i < 32 ==> abuf.[i] == buf.[i - 8]) /\
+    (i < 8 ==> abuf.[i] == false));
 
   assert(forall (i: nat{i < n + 16}). {:pattern Seq.index bbuf i}
-    (i >= 48 ==> Seq.index bbuf i == Seq.index buf (i - 16)) /\
+    (i >= 48 ==> bbuf.[i] == buf.[i - 16]) /\
     (i >= 40 /\ i < 48 ==> xor_status #n #16 bbuf buf a i 40) /\
     (i >= 32 /\ i < 40 ==> xor_status #n #16 bbuf buf b i 32) /\
-    (i >= 16 /\ i < 32 ==> Seq.index bbuf i == Seq.index buf (i - 16)) /\
-    (i < 16 ==> Seq.index bbuf i == false));
+    (i >= 16 /\ i < 32 ==> bbuf.[i] == buf.[i - 16]) /\
+    (i < 16 ==> bbuf.[i] == false));
 
   assert(forall (i: nat{i < n + 24}). {:pattern Seq.index cbuf i}
     (i >= 56 ==> Seq.index cbuf i == Seq.index buf (i - 24)) /\
     (i >= 48 /\ i < 56 ==> xor_status #n #24 cbuf buf a i 48) /\
     (i >= 40 /\ i < 48 ==> xor_status #n #24 cbuf buf b i 40) /\
     (i >= 32 /\ i < 40 ==> xor_status #n #24 cbuf buf c i 32) /\
-    (i >= 24 /\ i < 32 ==> Seq.index cbuf i == Seq.index buf (i - 24)) /\
-    (i < 24 ==> Seq.index cbuf i == false));
+    (i >= 24 /\ i < 32 ==> cbuf.[i] == buf.[i - 24]) /\
+    (i < 24 ==> cbuf.[i] == false));
 
   assert(forall (i: nat{i < n + 32}). {:pattern Seq.index dbuf i}
-    (i >= 64 ==> Seq.index dbuf i == Seq.index buf (i - 32)) /\
+    (i >= 64 ==> dbuf.[i] == buf.[i - 32]) /\
     (i >= 56 /\ i < 64 ==> xor_status #n #32 dbuf buf a i 56) /\
     (i >= 48 /\ i < 56 ==> xor_status #n #32 dbuf buf b i 48) /\
     (i >= 40 /\ i < 48 ==> xor_status #n #32 dbuf buf c i 40) /\
     (i >= 32 /\ i < 40 ==> xor_status #n #32 dbuf buf d i 32) /\
-    (i < 32 ==> Seq.index dbuf i == false));
+    (i < 32 ==> dbuf.[i] == false));
 
   assert(Seq.equal buf' dbuf)
 
@@ -531,14 +731,14 @@ let crc32_data_to_bits_32bit_aux''
   }): Lemma
   (ensures forall (i: nat{i < 64}). {:pattern Seq.index r' i}
     (i >= 56 ==> Seq.index r' i == (UInt.nth (U8.v a) (i - 56) <> true)) /\
-    (i >= 48 /\ i < 56 ==> Seq.index r' i == (UInt.nth (U8.v b) (i - 48) <> true)) /\
-    (i >= 40 /\ i < 48 ==> Seq.index r' i == (UInt.nth (U8.v c) (i - 40) <> true)) /\
-    (i >= 32 /\ i < 40 ==> Seq.index r' i == (UInt.nth (U8.v d) (i - 32) <> true)) /\
-    (i < 32 ==> Seq.index r' i == false)) = ()
+    (i >= 48 /\ i < 56 ==> r'.[i] == (UInt.nth (U8.v b) (i - 48) <> true)) /\
+    (i >= 40 /\ i < 48 ==> r'.[i] == (UInt.nth (U8.v c) (i - 40) <> true)) /\
+    (i >= 32 /\ i < 40 ==> r'.[i] == (UInt.nth (U8.v d) (i - 32) <> true)) /\
+    (i < 32 ==> r'.[i] == false)) = ()
 
 let crc32_data_to_bits_32bit_aux'''
   (#a #b #c #d: U8.t)
-  (m: nat{m > 0})
+  (m: pos)
   (data: Seq.seq U8.t{Seq.length data == m})
   (buf: BV.bv_t (32 + m * 8){buf == crc32_data_to_bits m data})
   (r: crc32_data_dword a b c d)
@@ -546,12 +746,12 @@ let crc32_data_to_bits_32bit_aux'''
     res == zero_vec_l 32 ((zero_vec_r (8 * m) (UInt.to_vec (U32.v r))) +@ buf)
   }): Lemma
   (ensures forall (i: nat{i < 64 + m * 8}). {:pattern Seq.index res i}
-    (i >= 64 ==> Seq.index res i == Seq.index buf (i - 32)) /\
+    (i >= 64 ==> res.[i] == buf.[i - 32]) /\
     (i >= 56 /\ i < 64 ==> xor_status #(32 + m * 8) #32 res buf a i 56) /\
     (i >= 48 /\ i < 56 ==> xor_status #(32 + m * 8) #32 res buf b i 48) /\
     (i >= 40 /\ i < 48 ==> xor_status #(32 + m * 8) #32 res buf c i 40) /\
     (i >= 32 /\ i < 40 ==> xor_status #(32 + m * 8) #32 res buf d i 32) /\
-    (i < 32 ==> Seq.index res i == false)) = ()
+    (i < 32 ==> res.[i] == false)) = ()
 
 #set-options "--z3rlimit 400 --fuel 1 --ifuel 0"
 let crc32_data_to_bits_unfold'
@@ -619,3 +819,10 @@ let crc32_data_to_bits_32bit #a #b #c #d m data buf r =
 
     assert(Seq.equal r' (crc32_data_to_bits 4 s))
   end
+
+let crc32_matched_xor_inv_3 m data crc =
+  let bits = crc32_data_to_bits m data in
+  let vcrc = UInt.to_vec (U32.v crc) in
+  let mask = zero_vec_r (8 * m) (BV.ones_vec #32) in
+  poly_mod_small #(32 + 8 * m) mask;
+  poly_mod_add bits mask
