specs/Spec.CRC32.Bits.fsti
@@ -4,70 +4,90 @@ module B = LowStar.Buffer
 module BV = FStar.BitVector
 module HS = FStar.HyperStack
 module Math = FStar.Math.Lib
-module Seq = FStar.Seq
 module U8 = FStar.UInt8
 module U32 = FStar.UInt32
 module UInt = FStar.UInt
 
 open FStar.Mul
+open FStar.Seq
 open Lib.Seq
 open Lib.UInt
 
-let rec logxor_vec_comm (#n: nat{n > 0}) (a b: BV.bv_t n): Lemma
+let rec logxor_vec_comm (#n: pos) (a b: BV.bv_t n): Lemma
   (ensures BV.logxor_vec a b == BV.logxor_vec b a)
   [SMTPat (BV.logxor_vec a b)] =
   match n with
   | 1 -> ()
   | _ -> let c = BV.logxor_vec a b in
     let c' = BV.logxor_vec b a in
-    assert_norm(Seq.index c 0 == Seq.index c' 0);
+    assert_norm(c.[0] == c'.[0]);
     logxor_vec_comm #(n - 1) (Seq.tail a) (Seq.tail b)
 
+let logxor_vec_assoc (#n: pos) (a b c: BV.bv_t n): Lemma
+  (ensures BV.logxor_vec (BV.logxor_vec a b) c == BV.logxor_vec a (BV.logxor_vec b c))
+  [SMTPat (BV.logxor_vec (BV.logxor_vec a b) c); 
+   SMTPat (BV.logxor_vec a (BV.logxor_vec b c))] =
+  assert(Seq.equal (BV.logxor_vec (BV.logxor_vec a b) c) (BV.logxor_vec a (BV.logxor_vec b c)))
+
+let logxor_vec_zero (#n: pos) (a: BV.bv_t n): Lemma
+  (ensures (BV.logxor_vec a (BV.zero_vec #n)) == a)
+  [SMTPat (BV.logxor_vec a (BV.zero_vec #n))] =
+    let z = BV.zero_vec #n in
+    let x = BV.logxor_vec a z in
+    assert_norm(forall (i: nat) (v: BV.bv_t n). i < n ==> v.[i] = v.[i] <> false);
+    assert_norm(Seq.equal x a)
+
+let logxor_vec_self (#n: pos) (a b: BV.bv_t n): Lemma
+  (requires a == b)
+  (ensures BV.logxor_vec a b == BV.zero_vec #n)
+  [SMTPat (BV.logxor_vec #n a b)] =
+  assert(Seq.equal (BV.logxor_vec a b) (BV.zero_vec #n))
+
 [@"opaque_to_smt"]
-let zero_vec_l (#n: nat{n > 0}) (m: nat) (a: BV.bv_t n): Tot (res: BV.bv_t (n + m){
+let zero_vec_l (#n: pos) (m: nat) (a: BV.bv_t n): Tot (res: BV.bv_t (n + m){
   (m == 0 ==> a == res) /\
-  (forall (i: nat{i < n + m}). {:pattern Seq.index res i}
-    (i < m ==> Seq.index res i == false) /\
-    (i >= m /\ i < n + m ==> Seq.index res i == Seq.index a (i - m)))
+  (forall (i: nat{i < n + m}). {:pattern res.[i]}
+    (i < m ==> res.[i] == false) /\
+    (i >= m /\ i < n + m ==> res.[i] == a.[i - m]))
 }) =
   match m with
   | 0 -> a
-  | _ -> Seq.append (BV.zero_vec #m) a
+  | _ -> (BV.zero_vec #m) @| a
 
 [@"opaque_to_smt"]
-let zero_vec_r (#n: nat{n > 0}) (m: nat) (a: BV.bv_t n): Tot (res: BV.bv_t (n + m){
+let zero_vec_r (#n: pos) (m: nat) (a: BV.bv_t n): Tot (res: BV.bv_t (n + m){
   (m == 0 ==> a == res) /\
-  (forall (i: nat{i < n + m}). {:pattern Seq.index res i}
-    (i < n ==> Seq.index res i == Seq.index a i) /\ 
-    ((i >= n /\ i < n + m) ==> Seq.index res i == false))
+  (forall (i: nat{i < n + m}). {:pattern res.[i]}
+    (i < n ==> res.[i] == a.[i]) /\ 
+    (i >= n /\ i < n + m ==> res.[i] == false))
 }) =
   match m with
   | 0 -> a
-  | _ -> Seq.append a (BV.zero_vec #m)
+  | _ -> a @| (BV.zero_vec #m)
 
 [@"opaque_to_smt"]
-let ones_vec_l (#n: nat{n > 0}) (m: nat) (a: BV.bv_t n): Tot (res: BV.bv_t (n + m){
+let ones_vec_l (#n: pos) (m: nat) (a: BV.bv_t n): Tot (res: BV.bv_t (n + m){
   (m == 0 ==> a == res) /\
-  (forall (i: nat{i < n + m}). {:pattern Seq.index res i}
-    (i < m ==> Seq.index res i == true) /\
-    (i >= m /\ i < n + m ==> Seq.index res i == Seq.index a (i - m)))
+  (forall (i: nat{i < n + m}). {:pattern res.[i]}
+    (i < m ==> res.[i] == true) /\
+    (i >= m /\ i < n + m ==> res.[i] == a.[i - m]))
 }) =
   match m with
   | 0 -> a
-  | _ -> Seq.append (BV.ones_vec #m) a
+  | _ -> (BV.ones_vec #m) @| a
 
 [@"opaque_to_smt"]
-let ones_vec_r (#n: nat{n > 0}) (m: nat) (a: BV.bv_t n): Tot (res: BV.bv_t (n + m){
+let ones_vec_r (#n: pos) (m: nat) (a: BV.bv_t n): Tot (res: BV.bv_t (n + m){
   (m == 0 ==> a == res) /\
-  (forall (i: nat{i < n + m}). {:pattern Seq.index res i}
-    (i < n ==> Seq.index res i == Seq.index a i) /\
-    (i >= n /\ i < n + m ==> Seq.index res i == true))
+  (forall (i: nat{i < n + m}). {:pattern res.[i]}
+    (i < n ==> res.[i] == a.[i]) /\
+    (i >= n /\ i < n + m ==> res.[i] == true))
 }) =
   match m with
   | 0 -> a
-  | _ -> Seq.append a (BV.ones_vec #m)
+  | _ -> a @| (BV.ones_vec #m)
 
-let lemma_vec_padding_zero (#n: nat{n > 0}) (s: BV.bv_t n): Lemma
+let lemma_vec_padding_zero (#n: pos) (s: BV.bv_t n): Lemma
   (ensures zero_vec_l 0 s == s /\ zero_vec_r 0 s == s /\
     ones_vec_l 0 s == s /\ ones_vec_r 0 s == s)
   [SMTPat (zero_vec_l 0 s); SMTPat (zero_vec_r 0 s);
@@ -77,16 +97,16 @@ let lemma_vec_padding_zero (#n: nat{n > 0}) (s: BV.bv_t n): Lemma
   assert(Seq.equal s (ones_vec_l 0 s));
   assert(Seq.equal s (ones_vec_r 0 s))
 
-let zero_vec_l_app (#n: nat{n > 0}) (a: BV.bv_t n) (m l: nat): Lemma
+let zero_vec_l_app (#n: pos) (a: BV.bv_t n) (m l: nat): Lemma
   (ensures zero_vec_l l (zero_vec_l m a) == zero_vec_l (m + l) a) =
   assert(Seq.equal (zero_vec_l l (zero_vec_l m a)) (zero_vec_l (m + l) a))
 
-unfold let gf2_plus (#n: nat{n > 0}) (a b: BV.bv_t n) : Tot (BV.bv_t n) =
+unfold let gf2_plus (#n: pos) (a b: BV.bv_t n) : Tot (BV.bv_t n) =
   BV.logxor_vec a b
 
 let (+@) #n = gf2_plus #n
 
-unfold let gf2_sub (#n: nat{n > 0}) (a b: BV.bv_t n) : Tot (BV.bv_t n) =
+unfold let gf2_sub (#n: pos) (a b: BV.bv_t n) : Tot (BV.bv_t n) =
   BV.logxor_vec a b
 
 let (-@) #n = gf2_sub #n
@@ -99,13 +119,13 @@ let gf2_polynomial32 = unsnoc gf2_polynomial
 
 type crc32_polynomial = res: U32.t{
   let res' = U32.v res in
-  forall i. UInt.nth res' i == Seq.index gf2_polynomial32 i
+  forall i. UInt.nth res' i == gf2_polynomial32.[i]
 }
 
 unfold let poly (n: nat{n >= 33}): Tot (p: BV.bv_t n{
-  Seq.index p (n - 1) == true
+  p.[n - 1] == true
 }) =
-  assert(Seq.index gf2_polynomial 32 == true);
+  assert(gf2_polynomial.[32] == true);
   zero_vec_l #33 (n - 33) gf2_polynomial
 
 let poly_xor (#n: nat{n >= 32}) (a: BV.bv_t n): Tot (res: BV.bv_t n{
@@ -130,25 +150,34 @@ val poly_mod_zero: #n: nat{n > 32} -> a: BV.bv_t n {a == BV.zero_vec #n} -> Lemm
 val poly_mod_add: #n: nat{n > 32} -> a: BV.bv_t n -> b: BV.bv_t n -> Lemma
   (ensures (poly_mod a) +@ (poly_mod b) == poly_mod (a +@ b))
 
-val poly_mod_zero_prefix: #n: nat{n > 32} -> a: BV.bv_t n -> m: nat{m > 0} -> Lemma
+val poly_mod_zero_prefix: #n: nat{n > 32} -> a: BV.bv_t n -> m: pos -> Lemma
   (ensures poly_mod (zero_vec_l m (poly_mod a)) == poly_mod (zero_vec_l m a))
 
-val poly_mod_zero_suffix: #n: nat{n >= 32} -> a: BV.bv_t n -> m: nat{m > 0} -> Lemma
+val poly_mod_zero_suffix: #n: nat{n >= 32} -> a: BV.bv_t n -> m: pos -> Lemma
   (ensures
     (n == 32 ==> poly_mod (zero_vec_r m a) == a) /\
     (n > 32 ==> poly_mod (zero_vec_r m a) == poly_mod a))
 
-unfold let poly_mod_correct (nzeros: nat{nzeros > 0}) (d res: U32.t) =
+#push-options "--fuel 1 --ifuel 1"
+let rec poly_mod_small (#m: nat{m > 32}) (vec: BV.bv_t m): Lemma
+  (requires forall i. i >= 32 ==> vec.[i] == false)
+  (ensures Seq.equal (poly_mod vec) (Seq.slice vec 0 32)) =
+  match m with
+  | 33 -> ()
+  | _ -> poly_mod_small #(m - 1) (Seq.slice vec 0 (m - 1))
+#pop-options
+
+unfold let poly_mod_correct (nzeros: pos) (d res: U32.t) =
   let d' = zero_vec_l nzeros (UInt.to_vec (U32.v d)) in
   forall i. {:pattern UInt.nth (U32.v res) i}
-    UInt.nth (U32.v res) i == Seq.index (poly_mod d') i
+    UInt.nth (U32.v res) i == (poly_mod d').[i]
 
-unfold let poly_mod_u32 (nzeros: nat{nzeros > 0}) (d: U32.t) =
+unfold let poly_mod_u32 (nzeros: pos) (d: U32.t) =
   poly_mod (zero_vec_l nzeros (UInt.to_vec (U32.v d)))
 
 val large_table_val_aux:
     i: U32.t{U32.v i < 256}
-  -> nzeros: nat{nzeros > 0}
+  -> nzeros: pos
   -> p: U32.t
   -> p': U32.t
   -> p'': U32.t
@@ -159,31 +188,24 @@ val large_table_val_aux:
     p'' == U32.shift_right p 8ul)
   (ensures poly_mod_correct (nzeros + 8) i (U32.logxor p' p''))
 
-let poly_mod_correct_eq (nzeros: nat{nzeros > 0}) (d res: U32.t): Lemma
+let poly_mod_correct_eq (nzeros: pos) (d res: U32.t): Lemma
   (requires poly_mod_correct nzeros d res)
   (ensures poly_mod_u32 nzeros d == UInt.to_vec (U32.v res)) =
   let open U32 in
-  assert(forall i. UInt.nth (v res) i == Seq.index (UInt.to_vec (v res)) i);
+  assert(forall i. UInt.nth (v res) i == (UInt.to_vec (v res)).[i]);
   assert(Seq.equal (poly_mod (zero_vec_l nzeros (UInt.to_vec (U32.v d)))) (UInt.to_vec (v res)))
 
-type table_buf = buf: B.buffer U32.t{B.length buf == 256}
+type table_buf = B.lbuffer U32.t 256
 
-let sub_table_correct
-  (j: nat{j <= 256})
-  (nzeros: nat{nzeros > 0})
-  (h: HS.mem)
-  (buf: table_buf) =
-  (B.live h buf) /\
-  (forall i. i < j ==>
-  poly_mod_correct nzeros (U32.uint_to_t i) (Seq.index (B.as_seq h buf) i))
+let sub_table_correct (j: nat{j <= 256}) (nzeros: pos) (h: HS.mem) (buf: table_buf) =
+  B.live h buf /\
+  (forall i. i < j ==> poly_mod_correct nzeros (U32.uint_to_t i) ((B.as_seq h buf).[i]))
 
-let table_correct
-  (nzeros: nat{nzeros > 0})
-  (h: HS.mem)
-  (buf: B.buffer U32.t{B.length buf == 256}) = sub_table_correct (B.length buf) nzeros h buf
+let table_correct (nzeros: pos) (h: HS.mem) (buf: table_buf) =
+  sub_table_correct 256 nzeros h buf
 
 private let rec seq_append_index_l (#t: Type) (a b: Seq.seq t): Lemma
-  (ensures forall i. i < Seq.length a ==> Seq.index a i == Seq.index (Seq.append a b) i)
+  (ensures forall i. i < Seq.length a ==> a.[i] == (a @| b).[i])
   (decreases Seq.length a) =
   match Seq.length a with
   | 0 -> ()
@@ -195,14 +217,13 @@ type crc32_buf_len = n: nat{n == 0 \/ n > 32}
 let crc32_append_8bit (#n: nat{n == 0 \/ n > 32}) (buf: BV.bv_t n) (b: U8.t):
   Tot (BV.bv_t (if n = 0 then 40 else n + 8)) =
   let v' = UInt.to_vec (U8.v b) in
-  let open Seq in
   if n = 0 then
     zero_vec_l 8 (BV.ones_vec #32 +@ (BV.zero_vec #24 @| v'))
   else
     let padding = (BV.zero_vec #24) @| v' @| (BV.zero_vec #(n - 32)) in
     zero_vec_l 8 (buf +@ padding)
 
-let rec crc32_data_to_bits_cont
+private let rec crc32_data_to_bits_cont
   (#n: crc32_buf_len) (m: nat)
   (data: Seq.seq U8.t {Seq.length data == m})
   (buf: BV.bv_t n):
@@ -225,15 +246,33 @@ unfold let crc32_data_to_bits (m: nat) (data: Seq.seq U8.t {Seq.length data == m
   Tot (BV.bv_t (if m = 0 then 0 else 32 + 8 * m)) =
   crc32_data_to_bits_cont #0 m data (Seq.empty #bool)
 
+let rec data_bits_rev (data: Seq.seq U8.t): Tot (res: BV.bv_t (Seq.length data * 8) {
+  forall (i: nat{i < Seq.length data}). Seq.equal
+    (Seq.slice res (i * 8) (i * 8 + 8))
+    (UInt.to_vec (U8.v data.[Seq.length data - 1 - i]))
+}) (decreases Seq.length data) =
+  match Seq.length data with
+  | 0 -> Seq.empty #bool
+  | _ -> data_bits_rev (Seq.tail data) @| (UInt.to_vec (U8.v (Seq.head data)))
+
+val data_bits_rev_app: s1: Seq.seq U8.t -> s2: Seq.seq U8.t -> Lemma
+  (ensures (data_bits_rev s2) @| data_bits_rev s1 == data_bits_rev (s1 @| s2))
+  (decreases length s2)
+
 #set-options "--z3rlimit 120 --z3seed 1"
 val crc32_data_to_bits_append:
      m1: nat
   -> m2: nat
   -> s1: Seq.seq U8.t{Seq.length s1 == m1}
   -> s2: Seq.seq U8.t{Seq.length s2 == m2}
-  -> Lemma (ensures crc32_data_to_bits_cont
-     #(if m1 > 0 then 32 + 8 * m1 else 0) m2 s2 (crc32_data_to_bits m1 s1) == 
-    crc32_data_to_bits (m1 + m2) (Seq.append s1 s2))
+  -> Lemma (ensures crc32_data_to_bits_cont m2 s2 (crc32_data_to_bits m1 s1) == 
+    crc32_data_to_bits (m1 + m2) (s1 @| s2))
+
+val crc32_data_to_bits_rev: n: pos -> data: Seq.seq U8.t -> Lemma
+  (requires Seq.length data == n)
+  (ensures crc32_data_to_bits n data == 
+    (zero_vec_l (n * 8) (BV.ones_vec #32)) +@
+    (zero_vec_l 32 (data_bits_rev data)))
 
 type crc32_data_dword (a b c d: U8.t) = res: U32.t{
   let a' = UInt.to_vec (U8.v a) in
@@ -241,11 +280,11 @@ type crc32_data_dword (a b c d: U8.t) = res: U32.t{
   let c' = UInt.to_vec (U8.v c) in
   let d' = UInt.to_vec (U8.v d) in
   let r' = UInt.to_vec (U32.v res) in
-  forall (i: nat{i < 32}). {:pattern Seq.index r' i}
-    (i >= 24 ==> Seq.index r' i == Seq.index a' (i - 24)) /\
-    ((16 <= i /\ i < 24) ==> Seq.index r' i == Seq.index b' (i - 16)) /\
-    ((8 <= i /\ i < 16) ==> Seq.index r' i == Seq.index c' (i - 8)) /\
-    (i < 8 ==> Seq.index r' i == Seq.index d' i)
+  forall (i: nat{i < 32}). {:pattern r'.[i]}
+    (i >= 24 ==> r'.[i] == a'.[i - 24]) /\
+    (16 <= i /\ i < 24 ==> r'.[i] == b'.[i - 16]) /\
+    (8 <= i /\ i < 16 ==> r'.[i] == c'.[i - 8]) /\
+    (i < 8 ==> r'.[i] == d'.[i])
 }
 
 unfold let crc32_dword_seq (a b c d: U8.t) =
@@ -267,7 +306,7 @@ val crc32_data_to_bits_32bit:
       crc32_data_to_bits 4 (crc32_dword_seq a b c d)) /\
     (m > 0 ==>
       zero_vec_l 32 ((zero_vec_r (8 * m) (UInt.to_vec (U32.v r))) +@ buf) ==
-      crc32_data_to_bits (m + 4) (Seq.append data (crc32_dword_seq a b c d))))
+      crc32_data_to_bits (m + 4) (data @| (crc32_dword_seq a b c d))))
 
 let crc32_matched (n: nat) (data: Seq.seq U8.t{Seq.length data == n}) (v: U32.t) (xor: bool) =
   let v' = if xor then
@@ -276,6 +315,17 @@ let crc32_matched (n: nat) (data: Seq.seq U8.t{Seq.length data == n}) (v: U32.t)
     UInt.to_vec (U32.v v) in
   (n == 0 ==> Seq.equal v' (BV.ones_vec #32)) /\
   (n > 0 ==> Seq.equal v' (poly_mod (crc32_data_to_bits n data)))
+
+let crc32_matched_zero (v: U32.t) (xor: bool): Lemma
+  (requires crc32_matched 0 (Seq.empty #U8.t) v xor)
+  (ensures
+    (xor == true ==> U32.v v == 0) /\
+    (xor == false ==> U32.v v == (pow2 32) - 1)) =
+  pow2_mask 32;
+  if xor = false then
+    assert(UInt.from_vec (UInt.to_vec (U32.v v)) == (pow2 32) - 1)
+  else
+    pow2_logxor (U32.v v)
 
 let crc32_matched_xor_inv_1 (m: nat) (data: Seq.seq U8.t{Seq.length data == m}) (crc: U32.t):
 Lemma
@@ -296,3 +346,15 @@ Lemma
     =={UInt.logxor_lemma_1 (v crc)}
     crc;
   }
+
+val crc32_matched_xor_inv_3:
+    m: pos
+  -> data: Seq.seq U8.t{Seq.length data == m}
+  -> crc: U32.t
+  -> Lemma
+  (requires crc32_matched m data crc true)
+  (ensures (
+    let bits = crc32_data_to_bits m data in
+    let vcrc = UInt.to_vec (U32.v crc) in
+    let mask = zero_vec_r (8 * m) (BV.ones_vec #32) in
+    Seq.equal vcrc (poly_mod (bits +@ mask))))
