specs/Spec.CRC32.Matrix.fst
@@ -6,76 +6,348 @@ module Bits = Spec.CRC32.Bits
 module HS = FStar.HyperStack
 module Seq = FStar.Seq
 module U32 = FStar.UInt32
+module U8 = FStar.UInt8
 module UInt = FStar.UInt
 
-let magic_matrix_pattern (nzeros: nat{nzeros > 0}) (i: nat{i < 32}):
-  res: BV.bv_t (nzeros + 32){
+open FStar.Seq
+open FStar.Mul
+open Lib.Seq
+open Lib.UInt
+
+type matrix_buf = B.lbuffer U32.t 32
+
+let magic_matrix_pattern (nzeros: pos) (i: nat{i < 32}):
+  Tot (res: BV.bv_t (nzeros + 32){
     forall j.
-      (j == nzeros + 31 - i ==> Seq.index res j == true) /\
-      (j <> nzeros + 31 - i ==> Seq.index res j == false)
-  } =
+      (j == nzeros + 31 - i ==> res.[j] == true) /\
+      (j <> nzeros + 31 - i ==> res.[j] == false)
+  }) =
   let zero_left = BV.zero_vec #(nzeros + 32 - i - 1) in
   let one = Bits.ones_vec_r 1 zero_left in
   Bits.zero_vec_r i one
 
-unfold let is_magic_matrix_elem (nzeros: nat{nzeros > 0}) (i: nat {i < 32}) (v: BV.bv_t 32) =
+/// An element in the magic matrix is the CRC-32 checksum of the magic matrix pattern.
+unfold let is_magic_matrix_elem (nzeros: pos) (i: nat {i < 32}) (v: BV.bv_t 32) =
   Bits.poly_mod (magic_matrix_pattern nzeros i) == v
 
 unfold let is_sub_matrix_buf
-  (h: HS.mem)
-  (len: nat{len <= 32})
-  (nzeros: nat{nzeros > 0})
-  (buf: B.buffer U32.t{B.length buf == 32}) =
+  (h: HS.mem) (len: nat{len <= 32}) (nzeros: pos) (buf: matrix_buf) =
   B.live h buf /\
   (forall (i: nat{i < len}).
-    is_magic_matrix_elem nzeros i (UInt.to_vec (U32.v (Seq.index (B.as_seq h buf) i))))
+    is_magic_matrix_elem nzeros i (UInt.to_vec (U32.v (B.as_seq h buf).[i])))
 
-unfold let is_matrix_buf
-  (h: HS.mem)
-  (nzeros: nat{nzeros > 0})
-  (buf: B.buffer U32.t{B.length buf == 32}) = is_sub_matrix_buf h 32 nzeros buf
+unfold let is_matrix_buf (h: HS.mem) (nzeros: pos) (buf: matrix_buf) =
+  is_sub_matrix_buf h 32 nzeros buf
 
-let bit_extract
-  (#len: nat{len > 0})
-  (n: BV.bv_t len)
-  (i: nat{0 <= i /\ i <= len - 1}):
-  Tot (res: BV.bv_t len {
+/// Extract the bit in the position len - i - 1.
+/// The result bit is wrapped with zeros.
+[@"opaque_to_smt"]
+let bit_extract (#len: pos) (n: BV.bv_t len) (i: nat{i < len}):
+ Tot (res: BV.bv_t len {
     forall j.
-      (j == len - i - 1 ==> Seq.index res j == Seq.index n j) /\
-      (j <> len - i - 1 ==> Seq.index res j == false)
+      (j == len - i - 1 ==> res.[j] == n.[j]) /\
+      (j <> len - i - 1 ==> res.[j] == false)
   }) =
   let zero_left = if i = len - 1 then Seq.empty #bool else BV.zero_vec #(len - i - 1) in
-  let bit = Seq.snoc zero_left (Seq.index n (len - i - 1)) in
+  let bit = Seq.snoc zero_left n.[len - i - 1] in
   Bits.zero_vec_r #(len - i) i bit
-  
-let rec bit_sum
-  (#len: nat{len > 0})
-  (n: BV.bv_t len)
-  (i: nat{0 <= i /\ i <= len - 1}):
+
+/// Keep last i + 1 bits the same as the sequence n, and add zero to the left of the
+/// result sequence.
+[@"opaque_to_smt"]
+let rec bit_sum (#len: pos) (n: BV.bv_t len) (i: nat{i < len}):
   Tot (res: BV.bv_t len {
     forall j.
-      (j >= len - i - 1 ==> Seq.index res j == Seq.index n j) /\
-      (j < len - i - 1 ==> Seq.index res j == false)
+      (j >= len - i - 1 ==> res.[j] == n.[j]) /\
+      (j < len - i - 1 ==> res.[j] == false)
   }) =
   match i with
   | 0 -> bit_extract n i
   | _ -> Bits.gf2_plus (bit_extract n i) (bit_sum n (i - 1))
 
-let bit_extract_eq_pattern
-  (#len: nat{len > 32})
-  (n: BV.bv_t len)
-  (i: nat{i < 32}): Lemma
-  (requires Seq.index n (len - 1 - i) == true)
+let bit_extract_eq_pattern (#len: nat{len > 32}) (n: BV.bv_t len) (i: nat{i < 32}): Lemma
+  (requires n.[len - 1 - i] == true)
   (ensures bit_extract n i == magic_matrix_pattern (len - 32) i) =
   assert(Seq.equal (bit_extract n i) (magic_matrix_pattern (len - 32) i))
 
-type sub_matrix_times_product (nzeros: nat{nzeros > 0}) (i: nat{i < 32}) (vec: U32.t) = 
+type sub_matrix_times_product (nzeros: pos) (i: nat{i < 32}) (vec: U32.t) = 
   res: U32.t{
     let vec' = Bits.zero_vec_l nzeros (UInt.to_vec (U32.v vec)) in
     UInt.to_vec (U32.v res) == Bits.poly_mod (bit_sum vec' i)
   }
 
-type matrix_times_product (nzeros: nat{nzeros > 0}) (vec: U32.t) =
+type matrix_times_product (nzeros: pos) (vec: U32.t) =
   sub_matrix_times_product nzeros 31 vec
 
-type matrix_buf = m: B.buffer U32.t{B.length m == 32}
+#set-options "--z3rlimit 1024 --fuel 0 --ifuel 0"
+private let crc32_expand_aux
+  (m: pos) (n: pos) (dm dn: Seq.seq U8.t): Lemma
+  (requires Seq.length dm == m /\ Seq.length dn == n)
+  (ensures (
+    let open Bits in
+    let mask_m = zero_vec_r (m * 8) (BV.ones_vec #32) in
+    let mask_n = zero_vec_r (n * 8) (BV.ones_vec #32) in
+    let mask_m' = zero_vec_l (m * 8) (BV.ones_vec #32) in
+    let mask_n' = zero_vec_l (n * 8) (BV.ones_vec #32) in
+    (zero_vec_l (n * 8) (mask_m' +@ zero_vec_l 32 (data_bits_rev dm))) +@
+    (zero_vec_l (n * 8) mask_m) +@
+    (zero_vec_r (m * 8) (mask_n' +@ zero_vec_l 32 (data_bits_rev dn))) +@
+    zero_vec_r (m * 8) mask_n ==
+    crc32_data_to_bits (n + m) (dm @| dn) +@
+    zero_vec_r ((n + m) * 8) (BV.ones_vec #32))) =
+  let open Bits in
+  let mask_m = zero_vec_r (m * 8) (BV.ones_vec #32) in
+  let mask_n = zero_vec_r (n * 8) (BV.ones_vec #32) in
+  let mask_m' = zero_vec_l (m * 8) (BV.ones_vec #32) in
+  let mask_n' = zero_vec_l (n * 8) (BV.ones_vec #32) in
+  calc (==) {
+    (zero_vec_l (n * 8) (mask_m' +@ zero_vec_l 32 (data_bits_rev dm))) +@
+    (zero_vec_l (n * 8) mask_m) +@
+    (zero_vec_r (m * 8) (mask_n' +@ zero_vec_l 32 (data_bits_rev dn))) +@
+    zero_vec_r (m * 8) mask_n;
+    =={
+      assert(Seq.equal
+        (zero_vec_l (n * 8) (mask_m' +@ zero_vec_l 32 (data_bits_rev dm)))
+        ((zero_vec_l (n * 8) mask_m') +@
+         (zero_vec_l (n * 8) (zero_vec_l 32 (data_bits_rev dm)))));
+      assert(Seq.equal
+        (zero_vec_r (m * 8) (mask_n' +@ zero_vec_l 32 (data_bits_rev dn)))
+        ((zero_vec_r (m * 8) mask_n') +@
+         (zero_vec_r (m * 8) (zero_vec_l 32 (data_bits_rev dn)))))
+    }
+    (zero_vec_l (n * 8) mask_m') +@
+    (zero_vec_l (n * 8) (zero_vec_l 32 (data_bits_rev dm))) +@
+    (zero_vec_l (n * 8) mask_m) +@
+    (zero_vec_r (m * 8) mask_n') +@
+    (zero_vec_r (m * 8) (zero_vec_l 32 (data_bits_rev dn))) +@
+    zero_vec_r (m * 8) mask_n;
+    =={
+      assert(Seq.equal (zero_vec_l (n * 8) mask_m) (zero_vec_r (m * 8) mask_n'));
+      Bits.logxor_vec_assoc
+        (zero_vec_l (n * 8) mask_m')
+        (zero_vec_l (n * 8) (zero_vec_l 32 (data_bits_rev dm)))
+        ((zero_vec_l (n * 8) mask_m) +@ (zero_vec_r (m * 8) mask_n'));
+      Bits.logxor_vec_self (zero_vec_l (n * 8) mask_m) (zero_vec_r (m * 8) mask_n');
+      Bits.logxor_vec_zero (zero_vec_l (n * 8) (zero_vec_l 32 (data_bits_rev dm)))
+    }
+    (zero_vec_l (n * 8) mask_m') +@
+    (zero_vec_l (n * 8) (zero_vec_l 32 (data_bits_rev dm))) +@
+    (zero_vec_r (m * 8) (zero_vec_l 32 (data_bits_rev dn))) +@
+    zero_vec_r (m * 8) mask_n;
+    =={
+      assert(Seq.equal
+        (zero_vec_l (n * 8) (zero_vec_l 32 (data_bits_rev dm)))
+        (zero_vec_l 32 (zero_vec_l (n * 8) (data_bits_rev dm))));
+      assert(Seq.equal
+        (zero_vec_r (m * 8) (zero_vec_l 32 (data_bits_rev dn)))
+        (zero_vec_l 32 (zero_vec_r (m * 8) (data_bits_rev dn))))
+    }
+    (zero_vec_l (n * 8) mask_m') +@
+    ((zero_vec_l 32 (zero_vec_l (n * 8) (data_bits_rev dm))) +@
+      (zero_vec_l 32 (zero_vec_r (m * 8) (data_bits_rev dn)))) +@
+    zero_vec_r (m * 8) mask_n;
+    =={
+      assert(Seq.equal
+        ((zero_vec_l 32 (zero_vec_l (n * 8) (data_bits_rev dm))) +@
+          (zero_vec_l 32 (zero_vec_r (m * 8) (data_bits_rev dn))))
+        (zero_vec_l 32 (
+          (zero_vec_l (n * 8) (data_bits_rev dm)) +@
+          (zero_vec_r (m * 8) (data_bits_rev dn))
+        )))
+    }
+    (zero_vec_l (n * 8) mask_m') +@
+    (zero_vec_l 32 (
+      (zero_vec_l (n * 8) (data_bits_rev dm)) +@
+      (zero_vec_r (m * 8) (data_bits_rev dn)))) +@
+    zero_vec_r (m * 8) mask_n;
+    =={
+      assert(Seq.equal
+        ((zero_vec_l (n * 8) (data_bits_rev dm)) +@ (zero_vec_r (m * 8) (data_bits_rev dn)))
+        ((data_bits_rev dn) @| data_bits_rev dm))
+    }
+    (zero_vec_l (n * 8) mask_m') +@
+    (zero_vec_l #((n + m) * 8) 32 ((data_bits_rev dn) @| data_bits_rev dm)) +@
+    zero_vec_r (m * 8) mask_n;
+    =={
+      data_bits_rev_app dm dn;
+      zero_vec_l_app (BV.ones_vec #32) (m * 8) (n * 8)
+    }
+    (zero_vec_l ((n + m) * 8) (BV.ones_vec #32)) +@
+    (zero_vec_l #((n + m) * 8) 32 (data_bits_rev (dm @| dn))) +@
+    zero_vec_r (m * 8) mask_n;
+    =={
+      crc32_data_to_bits_rev (n + m) (dm @| dn);
+      assert(Seq.equal
+        (zero_vec_r (m * 8) mask_n)
+        (zero_vec_r ((n + m) * 8) (BV.ones_vec #32)))
+    }
+    crc32_data_to_bits (n + m) (dm @| dn) +@ zero_vec_r ((n + m) * 8) (BV.ones_vec #32);
+  }
+
+private let crc32_matched_append_aux
+  (m: pos) (n: pos) (dm dn: Seq.seq U8.t) (cm cn: U32.t)
+  (cm': matrix_times_product (n * 8) cm): Lemma
+  (requires
+    Seq.length dm == m /\ Seq.length dn == n /\
+    Bits.crc32_matched m dm cm true /\ Bits.crc32_matched n dn cn true)
+  (ensures Bits.crc32_matched (m + n) (dm @| dn) (U32.logxor cm' cn) true) =
+  let open Spec.CRC32.Bits in
+  let vcm' = Bits.zero_vec_l (n * 8) (UInt.to_vec (U32.v cm)) in
+  let bm = crc32_data_to_bits m dm in
+  let bn = crc32_data_to_bits n dn in
+  let mask_m = zero_vec_r (m * 8) (BV.ones_vec #32) in
+  let mask_n = zero_vec_r (n * 8) (BV.ones_vec #32) in
+  let mask_m' = zero_vec_l (m * 8) (BV.ones_vec #32) in
+  let mask_n' = zero_vec_l (n * 8) (BV.ones_vec #32) in
+  let pm = zero_vec_l (n * 8) (bm +@ mask_m) in
+  let pn = zero_vec_r (m * 8) (bn +@ mask_n) in
+  calc (==) {
+    UInt.to_vec (U32.v cm');
+    =={assert(Seq.equal (bit_sum vcm' 31) vcm')}
+    poly_mod vcm';
+    =={crc32_matched_xor_inv_3 m dm cm}
+    poly_mod (zero_vec_l (n * 8) (poly_mod (bm +@ mask_m)));
+    =={poly_mod_zero_prefix (bm +@ mask_m) (n * 8)}
+    poly_mod pm;
+  };
+  UInt.logxor_lemma_1 (U32.v cn);
+  assert(U32.v cn `UInt.logxor` 0 == U32.v cn);
+  
+  UInt.logxor_self (UInt.ones 32);
+  assert(
+    (U32.v cn) `UInt.logxor` 0 ==
+    (U32.v cn) `UInt.logxor` ((UInt.ones 32) `UInt.logxor` (UInt.ones 32)));
+
+  calc (==) {
+    UInt.to_vec (U32.v cn);
+    =={
+      UInt.logxor_associative (U32.v cn) (UInt.ones 32) (UInt.ones 32);
+      pow2_mask 32
+    }
+    poly_mod bn +@ BV.ones_vec #32;
+    =={
+      poly_mod_small mask_n;
+      assert(Seq.equal (BV.ones_vec #32) (slice mask_n 0 32))
+    }
+    poly_mod bn +@ poly_mod mask_n;
+    =={poly_mod_add bn mask_n}
+    poly_mod (bn +@ mask_n);
+  };
+
+  assert(UInt.to_vec (U32.v cm' `UInt.logxor` U32.v cn) ==
+    poly_mod pm +@ poly_mod (bn +@ mask_n));
+
+  calc (==) {
+    poly_mod pm +@ poly_mod (bn +@ mask_n);
+    =={poly_mod_zero_suffix (bn +@ mask_n) (m * 8)}
+    poly_mod pm +@ poly_mod pn;
+    =={poly_mod_add pm pn}
+    poly_mod (pm +@ pn);
+    =={
+      assert(Seq.equal
+        (zero_vec_l (n * 8) (bm +@ mask_m))
+        ((zero_vec_l (n * 8) bm) +@ zero_vec_l (n * 8) mask_m));
+      assert(Seq.equal
+        (zero_vec_r (m * 8) (bn +@ mask_n))
+        ((zero_vec_r (m * 8) bn) +@ zero_vec_r (m * 8) mask_n))
+    }
+    poly_mod (
+      (zero_vec_l (n * 8) bm) +@ (zero_vec_l (n * 8) mask_m) +@
+      ((zero_vec_r (m * 8) bn) +@ zero_vec_r (m * 8) mask_n));
+    =={
+      Bits.logxor_vec_assoc
+        (zero_vec_l (n * 8) mask_m)
+        (zero_vec_r (m * 8) bn)
+        (zero_vec_r (m * 8) mask_n)
+    }
+    poly_mod (
+      (zero_vec_l (n * 8) bm) +@
+      (zero_vec_l (n * 8) mask_m) +@
+      (zero_vec_r (m * 8) bn) +@
+      zero_vec_r (m * 8) mask_n);
+    =={
+      crc32_data_to_bits_rev m dm;
+      crc32_data_to_bits_rev n dn
+    }
+    poly_mod (
+      (zero_vec_l (n * 8) (mask_m' +@ zero_vec_l 32 (data_bits_rev dm))) +@
+      (zero_vec_l (n * 8) mask_m) +@
+      (zero_vec_r (m * 8) (mask_n' +@ zero_vec_l 32 (data_bits_rev dn))) +@
+      zero_vec_r (m * 8) mask_n);
+    =={crc32_expand_aux m n dm dn}
+    poly_mod (
+      crc32_data_to_bits (n + m) (dm @| dn) +@
+      zero_vec_r ((n + m) * 8) (BV.ones_vec #32));
+    =={
+      poly_mod_add
+        (crc32_data_to_bits (n + m) (dm @| dn))
+        (zero_vec_r ((n + m) * 8) (BV.ones_vec #32))
+    }
+    poly_mod (crc32_data_to_bits (n + m) (dm @| dn)) +@
+    poly_mod (zero_vec_r ((n + m) * 8) (BV.ones_vec #32));
+    =={
+      poly_mod_zero_suffix (BV.ones_vec #32) ((n + m) * 8)
+    }
+    poly_mod (crc32_data_to_bits (n + m) (dm @| dn)) +@ BV.ones_vec #32;
+  }
+
+let crc32_matched_append
+  (m: nat) (n: pos) (dm dn: Seq.seq U8.t) (cm cn: U32.t)
+  (cm': matrix_times_product (n * 8) cm): Lemma
+  (requires
+    Seq.length dm == m /\ Seq.length dn == n /\
+    Bits.crc32_matched m dm cm true /\ Bits.crc32_matched n dn cn true)
+  (ensures Bits.crc32_matched (m + n) (dm @| dn) (U32.logxor cm' cn) true) =
+  if m = 0 then begin
+    let vcm' = Bits.zero_vec_l (n * 8) (UInt.to_vec (U32.v cm)) in
+    assert(Seq.equal (dm @| dn) dn);
+    calc (==) {
+      U32.v cm';
+      =={}
+      UInt.from_vec (UInt.to_vec (U32.v cm'));
+      =={}
+      UInt.from_vec (Bits.poly_mod (bit_sum vcm' 31));
+      =={
+        calc (==) {
+          vcm' <: BV.bv_t (n * 8 + 32);
+          =={}
+          (Bits.zero_vec_l (n * 8) (UInt.to_vec (U32.v cm))) <: BV.bv_t (n * 8 + 32);
+          =={
+            calc (==) {
+              UInt.to_vec (U32.v cm);
+              =={
+                Bits.crc32_matched_zero cm true;
+                assert(Seq.equal (UInt.to_vec (UInt.zero 32)) (UInt.to_vec (U32.v cm)))
+              }
+              UInt.to_vec (UInt.zero 32);
+              =={
+                assert(
+                  UInt.from_vec (UInt.to_vec (UInt.zero 32)) ==
+                  UInt.from_vec (BV.zero_vec #32))
+              }
+              BV.zero_vec #32;
+            }
+          }
+          (Bits.zero_vec_l (n * 8) (BV.zero_vec #32)) <: BV.bv_t (n * 8 + 32);
+          =={
+            assert(Seq.equal
+              (Bits.zero_vec_l (n * 8) (BV.zero_vec #32))
+              (BV.zero_vec #(n * 8 + 32)))
+          }
+          BV.zero_vec #(n * 8 + 32);
+        }
+      }
+      UInt.from_vec (Bits.poly_mod (bit_sum (BV.zero_vec #(n * 8 + 32)) 31));
+      =={
+        assert(Seq.equal
+          (bit_sum (BV.zero_vec #(n * 8 + 32)) 31)
+          (BV.zero_vec #(n * 8 + 32)))
+      }
+      UInt.from_vec (Bits.poly_mod (BV.zero_vec #(n * 8 + 32)));
+      =={Bits.poly_mod_zero (BV.zero_vec #(n * 8 + 32))}
+      UInt.from_vec (BV.zero_vec #32);
+      =={}
+      0;
+    }
+  end else
+    crc32_matched_append_aux m n dm dn cm cn cm'
